Implement Steel.Effect.Atomic

ulib/experimental/Steel.Effect.Atomic.fst
@@ -281,10 +281,128 @@ let bind_pure_steela_ (a:Type) (b:Type)
   (wp:pure_wp a)
   (#[@@ framing_implicit] pre:pre_t) (#[@@ framing_implicit] post:post_t b)
   (f:eqtype_as_type unit -> PURE a wp) (g:(x:a -> atomic_repr b opened_invariants o pre post))
-  : atomic_repr b opened_invariants o
+: Pure (atomic_repr b opened_invariants o
     pre
-    post
+    post)
+  (requires wp (fun _ -> True))
+  (ensures fun _ -> True)
   = fun _ ->
-    assume (wp (fun _ -> True));
     let x = f () in
     g x ()
+
+module Sems = Steel.Semantics.Hoare.MST
+module Ins = Steel.Semantics.Instantiate
+
+let bind_atomic_steel (a:Type) (b:Type)
+  (pre_f:pre_t) (post_f:post_t a) (is_ghost:observability)
+  (post_g:post_t b) (req_g:(x:a -> req_t (post_f x))) (ens_g:(x:a -> ens_t (post_f x) b post_g))
+  (f:atomic_repr a Set.empty is_ghost pre_f post_f) (g:(x:a -> Steel.Effect.repr b (post_f x) post_g (req_g x) (ens_g x)))
+: Steel.Effect.repr b pre_f post_g
+    (bind_req_atomicf_steelf req_g)
+    (bind_ens_atomicf_steelf ens_g)
+= fun _ ->
+    let m0:full_mem = NMST.get() in
+    let x = f () in
+    let m1:full_mem = NMST.get() in
+    assert (Sems.preserves_frame #Ins.state pre_f
+      (post_f x) m0 m1);
+    let y = g x () in
+    let m2:full_mem = NMST.get() in
+    Sems.preserves_frame_trans #Ins.state pre_f (post_f x) (post_g y) m0 m1 m2;
+    y
+
+let to_mst_preserves_frame (pre post:slprop) (m0 m1:full_mem)
+  : Lemma (requires preserves_frame Set.empty pre post m0 m1)
+          (ensures Sems.preserves_frame
+            #Ins.state pre post m0 m1)
+  = ()
+
+let bind_steelatomic_steelf (a:Type) (b:Type)
+  (o:observability)
+  (#[@@ framing_implicit] pre_f:pre_t) (#[@@ framing_implicit] post_f:post_t a)
+  (#[@@ framing_implicit] pre_g:a -> pre_t) (#[@@ framing_implicit] post_g:post_t b)
+  (#[@@ framing_implicit] req_g:(x:a -> req_t (pre_g x))) (#[@@ framing_implicit] ens_g:(x:a -> ens_t (pre_g x) b post_g))
+  (#[@@ framing_implicit] frame_f:slprop)
+  (#[@@ framing_implicit] p:squash (can_be_split_forall (fun x -> post_f x `star` frame_f) pre_g))
+  (f:atomic_repr a Set.empty o pre_f post_f)
+  (g:(x:a -> Steel.Effect.repr b (pre_g x) post_g (req_g x) (ens_g x)))
+: Steel.Effect.repr b
+    (pre_f `star` frame_f)
+    post_g
+    (bind_steelatomic_steelf_req req_g frame_f p)
+    (bind_steelatomic_steelf_ens ens_g frame_f p)
+= fun _ ->
+    let m0:full_mem = NMST.get() in
+    let x = f () in
+    let m1:full_mem = NMST.get() in
+    preserves_frame_extend Set.empty pre_f (post_f x) frame_f m0 m1;
+    preserves_frame_trans_equiv Set.empty (pre_f `star` frame_f) (post_f x `star` frame_f) (pre_g x) (pre_g x)
+      m0 m1 m1;
+    to_mst_preserves_frame (pre_f `star` frame_f) (pre_g x) m0 m1;
+    let y = g x () in
+    let m2:full_mem = NMST.get() in
+
+    Sems.preserves_frame_trans #Ins.state (pre_f `star` frame_f) (pre_g x) (post_g y) m0 m1 m2;
+    y
+
+let bind_steelatomic_steel (a:Type) (b:Type)
+  (o:observability)
+  (#[@@ framing_implicit] pre_f:pre_t) (#[@@ framing_implicit] post_f:post_t a)
+  (#[@@ framing_implicit] pre_g:a -> pre_t) (#[@@ framing_implicit] post_g:post_t b)
+  (#[@@ framing_implicit] req_g:(x:a -> req_t (pre_g x))) (#[@@ framing_implicit] ens_g:(x:a -> ens_t (pre_g x) b post_g))
+  (#[@@ framing_implicit] frame_f:slprop) (#[@@ framing_implicit] frame_g:slprop)
+  (#[@@ framing_implicit] p:squash (can_be_split_forall
+    (fun x -> post_f x `star` frame_f) (fun x -> pre_g x `star` frame_g)))
+  (f:atomic_repr a Set.empty o pre_f post_f)
+  (g:(x:a -> Steel.Effect.repr b (pre_g x) post_g (req_g x) (ens_g x)))
+: Steel.Effect.repr b
+    (pre_f `star` frame_f)
+    (fun y -> post_g y `star` frame_g)
+    (bind_steelatomic_steel_req req_g frame_f frame_g p)
+    (bind_steelatomic_steel_ens ens_g frame_f frame_g p)
+= fun _ ->
+    let m0:full_mem = NMST.get() in
+    let x = f () in
+    let m1:full_mem = NMST.get() in
+    preserves_frame_extend Set.empty pre_f (post_f x) frame_f m0 m1;
+    preserves_frame_trans_equiv Set.empty (pre_f `star` frame_f) (post_f x `star` frame_f) (pre_g x `star` frame_g) (pre_g x `star` frame_g)
+      m0 m1 m1;
+    to_mst_preserves_frame (pre_f `star` frame_f) (pre_g x `star` frame_g) m0 m1;
+    let y = g x () in
+    let m2:full_mem = NMST.get() in
+    Sems.preserves_frame_star #Ins.state (pre_g x) (post_g y) m1 m2 frame_g;
+
+    Sems.preserves_frame_trans #Ins.state (pre_f `star` frame_f) (pre_g x `star` frame_g) (post_g y `star` frame_g) m0 m1 m2;
+    y
+
+let subcomp_atomic_steel (a:Type)
+  (#[@@framing_implicit] pre_f:pre_t) (#[@@ framing_implicit] post_f:post_t a) (is_ghost:observability)
+  (f:atomic_repr a Set.empty is_ghost pre_f post_f)
+: Steel.Effect.repr a pre_f post_f (subcomp_req_atomic_steel a pre_f) (subcomp_ens_atomic_steel pre_f post_f)
+= fun _ -> f ()
+
+let lift_atomic_to_steelT f = f()
+let as_atomic_action f = SteelAtomic?.reflect f
+let new_invariant i p = SteelAtomic?.reflect (Steel.Memory.new_invariant i p)
+let with_invariant i f = SteelAtomic?.reflect (Steel.Memory.with_invariant i (reify (f())))
+let frame frame f = SteelAtomic?.reflect (Steel.Memory.frame frame (reify (f ())))
+let change_slprop p q proof = SteelAtomic?.reflect (Steel.Memory.change_slprop p q proof)
+
+let h_assert_atomic p = change_slprop p p (fun m -> ())
+let h_intro_emp_l p = change_slprop p (emp `star` p) (fun m -> emp_unit p; star_commutative p emp)
+let h_elim_emp_l p = change_slprop (emp `star` p) p (fun m -> emp_unit p; star_commutative p emp)
+let intro_pure #_ #p q = change_slprop p (p `star` pure q) (fun m -> emp_unit p; pure_star_interp p q m)
+let h_commute p q = change_slprop (p `star` q) (q `star` p) (fun m -> star_commutative p q)
+let h_assoc_left p q r = change_slprop ((p `star` q) `star` r) (p `star` (q `star` r)) (fun m -> star_associative p q r)
+let h_assoc_right p q r = change_slprop (p `star` (q `star` r)) ((p `star` q) `star` r) (fun m -> star_associative p q r)
+let intro_h_exists x p = change_slprop (p x) (h_exists p) (fun m -> Steel.Memory.intro_h_exists x p m)
+let intro_h_exists_erased x p = change_slprop (p x) (h_exists p) (fun m -> Steel.Memory.intro_h_exists (Ghost.reveal x) p m)
+let h_affine p q = change_slprop (p `star` q) p (fun m -> affine_star p q m)
+
+// open NMSTTotal
+// open MSTTotal
+
+let witness_h_exists #a #u #p () = SteelAtomic?.reflect (Steel.Memory.witness_h_exists p)
+let lift_h_exists_atomic #a #u p = SteelAtomic?.reflect (Steel.Memory.lift_h_exists #u p)
+let h_exists_cong_atomic p q = change_slprop (h_exists p) (h_exists q) (fun m -> h_exists_cong p q)
+let elim_pure #uses p = SteelAtomic?.reflect (Steel.Memory.elim_pure #uses p)
